fixed all combinators except flatMapD

Iterator/Combinators/Drop.lean
@@ -17,17 +17,9 @@ structure Drop (α : Type u) where
   inner : α
 
 instance [Monad m] [Iterator α m β] : SimpleIterator (Drop α) m β where
-  αInternal := Drop (IterState α m)
-  βInternal := Iterator.βInternal α m
-  αEquiv := {
-      hom it := { inner := Iterator.αEquiv.hom it.inner, remaining := it.remaining }
-      inv it := { inner := Iterator.αEquiv.inv it.inner, remaining := it.remaining }
-      hom_inv := by simp [Equiv.hom_inv]
-      inv_hom := by simp [Equiv.inv_hom] }
-  βEquiv := Iterator.βEquiv
   step it := matchStep (m := m) it.inner
       (fun it' b => match it.remaining with
-        | 0 => pure <| .yield ⟨0, it'⟩ (Iterator.βEquiv.hom b) ⟨⟩
+        | 0 => pure <| .yield ⟨0, it'⟩ b ⟨⟩
         | remaining' + 1 => pure <| .skip ⟨remaining', it'⟩ ⟨⟩)
       (fun it' => pure <| .skip ⟨it.remaining, it'⟩ ⟨⟩)
       (pure <| .done ⟨⟩)
@@ -58,10 +50,11 @@ _TODO_: prove `Productive`
 Currently, this combinator incurs an additional O(1) cost with each output of `it`, even when the iterator
 does not drop any elements anymore.
 -/
-def Iter.drop [Iterator α m β] [Monad m] (n : Nat) (it : Iter (α := α) m β) :=
+def Iter.drop [Iterator α m β] [Monad m] [ComputableUnivLE.{u, w}] {small : ComputableSmall.{w} α}
+    (n : Nat) (it : Iter (α := α) m β (small := small)) :=
   toIter (α := Drop α) m <| Drop.mk n it.inner
 
-def Drop.rel (m : Type w → Type w') [Iterator α m β] : Drop (IterState α m) → Drop (IterState α m) → Prop :=
+def Drop.rel (m : Type w → Type w') [Iterator α m β] : Drop α → Drop α → Prop :=
   InvImage FiniteIteratorWF.lt (finiteIteratorWF (m := m) ∘ Drop.inner)
 
 instance [Iterator α m β] [Monad m] [Finite α m] : SimpleIterator.Finite (Drop α) m where
