Iterator/Consumers.lean
@@ -5,89 +5,87 @@ Authors: Paul Reichert
 -/
 prelude
 import Iterator.Wrapper
-import Iterator.Combinators.MonadEval
 
-@[inline]
-def Iter.forIn {m n} [Monad m] [Monad n] [MonadEvalT m n] {α β γ} [Iterator α m β] [Finite α m]
+@[specialize]
+def Iter.forIn {m : Type w → Type w'} {n : Type w → Type w''} [Monad m] [Monad n] [MonadLiftT m n]
+    {α : Type u} {β : Type v} {γ : Type w}
+    {_ : Iterator α m β} [Finite α m] {_ : ComputableSmall.{w} α} [ComputableSmall.{w} β]
     (it : Iter (α := α) m β) (init : γ) (f : β → γ → n (ForInStep γ)) : n γ := do
-  let x : OverT n (IterStep.for m it) := MonadEvalT.monadEval <| Iterator.step it
-  match x.f (← x.el) with
+  let x : n it.LiftedStep := it.stepH.mapH (·.lift) |>.run
+  match ← x with
   | .yield it' b _ =>
-    match ← f b init with
+    match ← f (ComputableSmall.down b) init with
     | .yield c => it'.forIn c f
     | .done c => return c
   | .skip it' _ => it'.forIn init f
   | .done _ => return init
-termination_by finiteIteratorWF (m := m) it
+termination_by it.terminationByFinite
 
-instance {m} [Monad m] [Monad n] [MonadEvalT m n] {α β} [Iterator α m β] [Finite α m] :
+instance {m} [Monad m] [Monad n] [MonadLiftT m n] {α β} [Iterator α m β] [Finite α m] :
     ForIn n (Iter (α := α) m β) β where
   forIn := Iter.forIn
 
 @[specialize]
-def Iter.fold {m n} [Monad m] [Monad n] [MonadEvalT m n] {α β γ} [Iterator α m β] [Finite α m]
+def Iter.fold {m : Type w → Type w'} {n : Type w → Type w'} [Monad m] [Monad n] [MonadLiftT m n]
+    {α : Type u} {β : Type v} {γ : Type w} {_ : Iterator α m β} [Finite α m] {_ : ComputableSmall.{w} α} [ComputableSmall.{w} β]
     (f : γ → β → n γ) (init : γ) (it : Iter (α := α) m β) : n γ := do
-  let step : OverT n (IterStep.for m it) := MonadEvalT.monadEval <| Iterator.step it
-  match step.f (← step.el) with
-  | .yield it' b _ => it'.fold f (← f init b)
+  let step : n it.LiftedStep := it.stepH.mapH (·.lift) |>.run
+  match ← step with
+  | .yield it' b _ => it'.fold f (← f init (ComputableSmall.down b))
   | .skip it' _ => it'.fold f init
   | .done _ => return init
-termination_by finiteIteratorWF (m := m) it
+termination_by it.terminationByFinite
 
--- TODO: This may have performance problems because we use bindH and recursion so that
--- Lean won't be able to inline the `OverT` code.
 @[inline]
 def Iter.toArrayH {α : Type u} {m : Type w → Type w'} [Monad m] {β : Type v}
-    [Iterator α m β] [Finite α m] (it : Iter (α := α) m β) : OverT m (Array β) :=
-  go it #[]
+    {_ : Iterator α m β} [Finite α m] {_ : ComputableSmall.{w} α} [ComputableUnivLE.{v, w}] (it : Iter (α := α) m β) : CodensityT m (Array β) :=
+  (CodensityT.eval <| go it #[]).mapH ComputableSmall.down
 where
   @[specialize]
-  go [Monad m] [Finite α m] it a := do
-    let step := Iterator.step (m := m) it
-    step.bindH (match · with
-      | .yield it' b _ => go it' (a.push b)
+  go [Monad m] [Finite α m] it a : m (ComputableSmall.Lift.{w} (Array β)) := do
+    let step ← it.stepH.mapH (·.lift) |>.run
+    match step with
+      | .yield it' b _ => go it' (a.push <| ComputableSmall.down b)
       | .skip it' _ => go it' a
-      | .done _ => return a)
-  termination_by finiteIteratorWF (m := m) it
+      | .done _ => return ComputableSmall.up a
+  termination_by it.terminationByFinite
 
 @[inline]
 def Iter.toArray {α : Type u} {m : Type v → Type w} [Monad m] {β : Type v}
-    [Iterator α m β] [Finite α m] (it : Iter (α := α) m β) : m (Array β) :=
+    {_ : Iterator α m β} [Finite α m] {_ : ComputableSmall.{v} α} (it : Iter (α := α) m β) : m (Array β) :=
   go it #[]
 where
   @[specialize]
   go [Monad m] [Finite α m] it a := do
-    let step := Iterator.step it
-    match step.f (← step.el) with
+    match ← it.step with
     | .yield it' b _ => go it' (a.push b)
     | .skip it' _ => go it' a
     | .done _ => return a
-  termination_by finiteIteratorWF (m := m) it
+  termination_by it.terminationByFinite
 
 @[inline]
 def Iter.reverseToList {α : Type u} {m : Type v → Type w} [Monad m] {β : Type v}
-    [Iterator α m β] [Finite α m] (it : Iter (α := α) m β) : m (List β) :=
+    {_ : Iterator α m β} [Finite α m] {_ : ComputableSmall.{v} α} (it : Iter (α := α) m β) : m (List β) :=
   go it []
 where
   @[specialize]
   go [Finite α m] it bs := do
-    let step := Iterator.step it
-    match step.f (← step.el) with
+    match ← it.step with
     | .yield it' b _ => go it' (b :: bs)
     | .skip it' _ => go it' bs
     | .done _ => return bs
-  termination_by finiteIteratorWF (m := m) it
+  termination_by it.terminationByFinite
 
 @[inline]
 def Iter.toList {α : Type u} {m : Type v → Type w} [Monad m] {β : Type v}
-    [Iterator α m β] [Finite α m] (it : Iter (α := α) m β) : m (List β) :=
+    {_ : Iterator α m β} [Finite α m] {_ : ComputableSmall.{v} α} (it : Iter (α := α) m β) : m (List β) :=
   Array.toList <$> it.toArray
 
 @[specialize]
-def Iter.drain [Monad m] [Iterator α m β] [Finite α m] (it : Iter (α := α) m β) : m PUnit := do
-  let step := Iterator.step it
-  match step.f (← step.el) with
+def Iter.drain {α : Type u} {m : Type w → Type w'} {β : Type v} [Monad m]
+    {_ : Iterator α m β} [Finite α m] {_ : ComputableSmall α} (it : Iter (α := α) m β) : m PUnit := do
+  it.stepH _ (match · with
   | .yield it' _ _ => it'.drain
   | .skip it' _ => it'.drain
-  | .done _ => return ⟨⟩
-  termination_by finiteIteratorWF (m := m) it
+  | .done _ => return ⟨⟩)
+termination_by it.terminationByFinite
